BindDep.v
@@ -1,0 +1,111 @@
+Require Import
+  Coq.Sets.Ensembles.
+
+Require Import
+  Fiat.ADT
+  Fiat.ADTNotation.
+
+Require Import
+  Fiat.ADTRefinement
+  Fiat.ADTRefinement.BuildADTRefinements.
+
+Generalizable All Variables.
+
+Lemma refine_In `(H : In A ca a) : refine ca (ret a).
+Proof.
+  intros ??.
+  destruct H0.
+  exact H.
+Defined.
+
+Definition Bind_dep {A B : Type} (ca : Comp A)
+           (k : forall v : A, refine ca (ret v) -> Comp B) : Comp B :=
+  fun b : B =>
+    exists a : A, { H : In A ca a & In B (k a (refine_In H)) b }.
+
+Arguments Bind_dep {A B} ca k _.
+
+Global Opaque Bind_dep.
+
+Notation "`( a | H ) <- c ; k" :=
+  (Bind_dep c (fun a H => k))
+    (at level 81, right associativity,
+     format "'[v' `( a | H )  <-  c ; '/' k ']'") : comp_scope.
+
+Lemma refine_reveal_dep : forall A (c : Comp A) B (k : A -> Comp B),
+  refine (x <- c; k x) (`(x | H) <- c; k x).
+Proof.
+  intros.
+  intros x?.
+  destruct H.
+  exists x0.
+  destruct H.
+  split; trivial.
+Qed.
+
+Lemma refine_bind_dep_ret :
+  forall A a B (k : forall x : A, refine (ret a) (ret x) -> Comp B),
+  refine (`(x | H) <- ret a; k x H)
+         (k a (refine_In (ReturnComputes a))).
+Proof.
+  intros.
+  intros x?.
+  Local Transparent Bind_dep.
+  unfold Bind_dep.
+  exists a.
+  exists (ReturnComputes a).
+  exact H.
+Qed.
+
+Lemma refine_bind_dep_bind_ret :
+  forall A (c : Comp A) B (f : forall x : A, refine c (ret x) -> B)
+         C (k : B -> Comp C),
+    refine
+      (r_o' <- `(x|H) <- c;
+               ret (f x H);
+       k r_o')
+       (`(x|H) <- c;
+       k (f x H)).
+Proof.
+  intros.
+  intros ??.
+  destruct H.
+  destruct H.
+  eapply BindComputes.
+    Focus 2.
+    apply i.
+  eexists.
+  exists x0.
+  constructor.
+Qed.
+
+Lemma refine_bind_dep {A} (c : Comp A) B
+      (k : forall x : A, refine c (ret x) -> Comp B) :
+  forall x (H : refine c (ret x)),
+    refine (`(x | H) <- c; k x H)
+           (k x H).
+Proof.
+  intros.
+  exists x.
+  exists (H _ (ReturnComputes _)).
+  destruct (ReturnComputes x).
+  assert (refine_In (H x (In_singleton A x)) = H).
+    unfold refine_In.
+    extensionality z.
+    extensionality H1.
+    destruct H1.
+    reflexivity.
+  rewrite <- H1 in H0.
+  apply H0.
+Qed.
+
+Lemma refine_bind_dep_ignore {A} (c : Comp A) B (k : A -> Comp B) :
+  refine (`(x | _) <- c; k x) (x <- c; k x).
+Proof.
+  intros ??.
+  destruct H.
+  destruct H.
+  exists x.
+  exists H.
+  exact H0.
+Qed.
