FromADT.v
@@ -1,0 +1,131 @@
+Require Import
+  Fiat.ADT
+  Fiat.ADTNotation.
+
+Require Import
+  Fiat.ADTRefinement
+  Fiat.ADTRefinement.BuildADTRefinements.
+
+Require Import
+  Here.LibExt
+  Here.BindDep
+  Here.ADTInduction.
+
+Definition fromADTConstructor'
+           {dSig : DecoratedADTSig}
+           (adt : DecoratedADT dSig)
+           (idxMap : BoundedIndex (ConstructorNames dSig)
+                       -> ConstructorIndex dSig)
+           (idx : BoundedIndex (ConstructorNames dSig)) :
+  forall (r : Rep adt),
+    fromConstructor (Constructors adt (idxMap idx)) r
+      -> fromADT adt r :=
+  ADTInduction.fromADTConstructor adt (idxMap idx).
+
+Arguments fromADTConstructor' {dSig} adt idxMap idx r _.
+
+Notation fromCons adt idx :=
+  (fromADTConstructor' adt (fun idx => ibound (indexb idx))
+                           {| bindex := idx |}).
+
+Lemma refine_computes_to {A} {c : Comp A} {v} :
+  c ↝ v -> refine c (ret v).
+Proof.
+  intros.
+  intros ??.
+  inv H0.
+  exact H.
+Qed.
+
+Lemma computes_to_refine {A} {c : Comp A} {v} :
+  refine c (ret v) -> c ↝ v.
+Proof. intros; exact (H _ (ReturnComputes _)). Qed.
+
+Tactic Notation "check" "constructor" constr(t) :=
+  simpl; intros;
+  apply t;
+  repeat match goal with
+    | [ H : refine _ (ret _) |- _ ] => apply computes_to_refine in H
+    | [ |- fromConstructor _ _ _ ] => eexists
+    | [ H : _ ↝ _ |- _ ↝ _ ] => exact H
+    | [ H : ?X |- ?X ] => exact H
+    end.
+
+Definition fromADTMethod'
+           {dSig : DecoratedADTSig}
+           (adt : DecoratedADT dSig)
+           (idxMap : BoundedIndex (MethodNames dSig) -> MethodIndex dSig)
+           (idx : BoundedIndex (MethodNames dSig)) :
+  forall (r r' : Rep adt),
+    fromADT adt r
+      -> fromMethod (Methods adt (idxMap idx)) r r'
+      -> fromADT adt r' :=
+  ADTInduction.fromADTMethod (adt:=adt) (idxMap idx).
+
+Arguments fromADTMethod' {dSig} adt idxMap idx r r' _ _.
+
+Notation fromMeth adt idx :=
+  (fromADTMethod' adt (fun idx => ibound (indexb idx)) {| bindex := idx |}).
+
+Tactic Notation "check" "method" constr(t) :=
+  simpl; intros;
+  apply t;
+  repeat match goal with
+    | [ H : _ * _ |- _ ] => destruct H; simpl in *
+    | [ H : refine _ (ret _) |- _ ] => apply computes_to_refine in H
+    | [ |- fromMethod _ _ _ ] => eexists
+    | [ |- fromMethod' _ _ ] => eexists
+    | [ H : _ ↝ _ |- _ ↝ _ ] => exact H
+    | [ H : ?X |- ?X ] => exact H
+    end.
+
+Lemma refine_constructor_fromADT
+      A (c : Comp (A)) (P : A -> Prop)
+      (f : forall v : A, refine c (ret v) -> P v) :
+   refine (r_o' <- c;
+           {r_n0 : {r : A | P r} | r_o' = ` r_n0})
+          (`(r_o' | H) <- c;
+           ret (exist _ r_o' (f r_o' H))).
+Proof.
+  intros x?.
+  destruct H.
+  exists x0.
+  destruct H.
+  split; trivial.
+  destruct i.
+  esplit.
+Qed.
+
+Lemma refine_method_fromADT
+      A B (c : Comp (A * B)) (P : A -> Prop)
+      (f : forall v : A * B, refine c (ret v) -> P (fst v)) :
+   refine (r_o' <- c;
+           r_n' <- {r_n0 : {r : A | P r} | fst r_o' = ` r_n0};
+           ret (r_n', snd r_o'))
+          (`(r_o' | H) <- c;
+           ret (exist _ (fst r_o') (f r_o' H),
+                snd r_o')).
+Proof.
+  intros x?.
+  destruct H.
+  exists x0.
+  destruct H.
+  split; trivial.
+  destruct i.
+  esplit; split.
+    Focus 2.
+    constructor.
+  constructor.
+Qed.
+
+Ltac resolve_constructor m H0 :=
+  subst; subst_evars;
+  etransitivity;
+  [ apply (refine_constructor_fromADT _ (c:=m) H0)
+  | finish honing].
+
+Ltac resolve_method r_n m H0 :=
+  subst; subst_evars;
+  etransitivity;
+  [ apply (refine_method_fromADT _ (c:=m) H0)
+  | finish honing].
