HeapADT.v
@@ -1,0 +1,101 @@
+Require Import
+  Coq.Sets.Ensembles
+  Coq.NArith.NArith
+  Fiat.ADT
+  Fiat.ADTNotation
+  Here.ADTInduction
+  Here.FromADT
+  Here.Heap.
+
+Section HeapADT.
+
+Variable Word8 : Type.
+Variable Zero  : Word8.
+
+Definition MemoryBlock := MemoryBlock Word8.
+Definition HeapSpec    := @HeapSpec Word8 Zero.
+
+Lemma empty_fromADT r :
+  refine (callCons HeapSpec emptyS) (ret r) -> fromADT HeapSpec r.
+Proof. check constructor (fromCons HeapSpec emptyS r). Qed.
+
+Open Scope N_scope.
+
+Lemma alloc_fromADT r :
+  fromADT HeapSpec r
+    -> forall (len : N | 0 < len) v,
+         refine (callMeth HeapSpec allocS r len) (ret v)
+    -> fromADT HeapSpec (fst v).
+Proof. intros; check method (fromMeth HeapSpec allocS r (fst v)). Qed.
+
+Lemma free_fromADT r :
+  fromADT HeapSpec r
+    -> forall (addr : N) v,
+         refine (callMeth HeapSpec freeS r addr) (ret v)
+    -> fromADT HeapSpec (fst v).
+Proof. intros; check method (fromMeth HeapSpec freeS r (fst v)). Qed.
+
+Lemma realloc_fromADT r :
+  fromADT HeapSpec r
+    -> forall (addr : N) (len : N | 0 < len) v,
+         refine (callMeth HeapSpec reallocS r addr len) (ret v)
+    -> fromADT HeapSpec (fst v).
+Proof. intros; check method (fromMeth HeapSpec reallocS r (fst v)). Qed.
+
+Lemma peek_fromADT r :
+  fromADT HeapSpec r
+    -> forall (addr : N) v,
+         refine (callMeth HeapSpec peekS r addr) (ret v)
+    -> fromADT HeapSpec (fst v).
+Proof. intros; check method (fromMeth HeapSpec peekS r (fst v)). Qed.
+
+Lemma poke_fromADT r :
+  fromADT HeapSpec r
+    -> forall (addr : N) w v,
+         refine (callMeth HeapSpec pokeS r addr w) (ret v)
+    -> fromADT HeapSpec (fst v).
+Proof. intros; check method (fromMeth HeapSpec pokeS r (fst v)). Qed.
+
+Lemma memcpy_fromADT r :
+  fromADT HeapSpec r
+    -> forall (addr : N) (addr2 : N) (len : N | 0 < len) v,
+         refine (callMeth HeapSpec memcpyS r addr addr2 len) (ret v)
+    -> fromADT HeapSpec (fst v).
+Proof. intros; check method (fromMeth HeapSpec memcpyS r (fst v)). Qed.
+
+Lemma memset_fromADT r :
+  fromADT HeapSpec r
+    -> forall (addr : N) (len : N | 0 < len) (w : Word8) v,
+         refine (callMeth HeapSpec memsetS r addr len w) (ret v)
+    -> fromADT HeapSpec (fst v).
+Proof. intros; check method (fromMeth HeapSpec memsetS r (fst v)). Qed.
+
+Require Import
+  Fiat.ADTRefinement
+  Fiat.ADTRefinement.BuildADTRefinements.
+
+Theorem HeapSpecADT : { adt : _ & refineADT HeapSpec adt }.
+Proof.
+  eexists.
+  hone representation using
+    (fun (or : Rep HeapSpec)
+         (nr : { r : Rep HeapSpec | fromADT HeapSpec r }) => or = ` nr).
+  resolve_constructor (@empty Word8 Zero) empty_fromADT.
+  resolve_method r_n (@alloc Word8 Zero (` r_n) d)
+                     (@alloc_fromADT _ (proj2_sig r_n) d).
+  resolve_method r_n (@free Word8 Zero (` r_n) d)
+                     (@free_fromADT _ (proj2_sig r_n) d).
+  resolve_method r_n (@realloc Word8 Zero (` r_n) d d0)
+                     (@realloc_fromADT _ (proj2_sig r_n) d d0).
+  resolve_method r_n (@peek Word8 Zero (` r_n) d)
+                     (@peek_fromADT _ (proj2_sig r_n) d).
+  resolve_method r_n (@poke Word8 Zero (` r_n) d d0)
+                     (@poke_fromADT _ (proj2_sig r_n) d d0).
+  resolve_method r_n (@memcpy Word8 Zero (` r_n) d d0 d1)
+                     (@memcpy_fromADT _ (proj2_sig r_n) d d0 d1).
+  resolve_method r_n (@memset Word8 Zero (` r_n) d d0 d1)
+                     (@memset_fromADT _ (proj2_sig r_n) d d0 d1).
+  apply reflexivityT.
+Defined.
+
+End HeapADT.
