Nomega.v
@@ -1,0 +1,187 @@
+Require Import
+  Fiat.ADT
+  Fiat.ADTNotation.
+
+Require Export
+  Coq.NArith.NArith
+  Omega.
+
+Require Export
+  Here.Decidable.
+
+Open Scope N_scope.
+
+Definition within (addr : N) (len : N) (a : N) : Prop :=
+  addr <= a < addr + len.
+
+Definition within_le (addr : N) (len : N) (a : N) : Prop :=
+  addr <= a <= addr + len.
+
+Lemma within_refl : forall addr len,
+  0 < len -> within addr len addr.
+Proof.
+  split; intros.
+    apply N.le_refl.
+  apply N.lt_add_pos_r.
+  assumption.
+Qed.
+
+Definition fits (addr1 len1 addr2 len2 : N) : Prop :=
+  within addr1 len1 addr2 /\ within addr1 len1 (addr2 + len2).
+
+Definition overlaps (addr len addr2 len2 : N) : Prop :=
+  addr < addr2 + len2 /\ addr2 < addr + len.
+
+Lemma overlaps_sym : forall addr1 len1 addr2 len2,
+  overlaps addr1 len1 addr2 len2 <-> overlaps addr2 len2 addr1 len1.
+Proof.
+  split; intros;
+  destruct H; split; assumption.
+Qed.
+
+Lemma overlaps_irr : forall addr len1 len2,
+  0 < len1 -> 0 < len2 -> overlaps addr len1 addr len2.
+Proof.
+  split; intros;
+  apply N.lt_add_pos_r; assumption.
+Qed.
+
+Ltac decisions :=
+  repeat
+    match goal with
+    | [ H : context [if ?B then _ else _] |- _ ] =>
+      let Heqe := fresh "Heqe" in
+      destruct B eqn:Heqe
+    | [ |- context [if ?B then _ else _] ] =>
+      let Heqe := fresh "Heqe" in
+      destruct B eqn:Heqe
+
+    | [ H : context[@IfDec_Then_Else _ _ _ _ _] |- _ ] =>
+      unfold IfDec_Then_Else in H; simpl in H
+    | [ |- context[@IfDec_Then_Else _ _ _ _ _] ] =>
+      unfold IfDec_Then_Else; simpl
+    end.
+
+Ltac undecide :=
+  repeat
+    match goal with
+    | [ H : (_ <? _)  = true  |- _ ] => apply N.ltb_lt in H
+    | [ H : (_ <? _)  = false |- _ ] => apply N.ltb_ge in H
+    | [ H : (_ <=? _) = true  |- _ ] => apply N.leb_le in H
+    | [ H : (_ <=? _) = false |- _ ] => apply N.leb_gt in H
+    | [ H : (_ =? _)  = true  |- _ ] => apply N.eqb_eq in H; subst
+    | [ H : (_ =? _)  = false |- _ ] => apply N.eqb_neq in H
+
+    | [ |- (_ <? _)  = true  ] => apply N.ltb_lt
+    | [ |- (_ <? _)  = false ] => apply N.ltb_ge
+    | [ |- (_ <=? _) = true  ] => apply N.leb_le
+    | [ |- (_ <=? _) = false ] => apply N.leb_gt
+    | [ |- (_ =? _)  = true  ] => apply N.eqb_eq
+    | [ |- (_ =? _)  = false ] => apply N.eqb_neq
+    end.
+
+Ltac nomega_reduce :=
+  repeat (
+    match goal with
+    | [ H : (_ && _)%bool = true |- _ ] =>
+      apply Bool.andb_true_iff in H; destruct H
+    | [ H : (_ && _)%bool = false |- _ ] =>
+      apply Bool.andb_false_iff in H; destruct H
+
+    | [ H : _ <  _ <  _ |- _ ] => destruct H
+    | [ H : _ <= _ <  _ |- _ ] => destruct H
+    | [ H : _ <  _ <= _ |- _ ] => destruct H
+    | [ H : _ <= _ <= _ |- _ ] => destruct H
+
+    | [ |- _ <  _ <  _ ] => split
+    | [ |- _ <= _ <  _ ] => split
+    | [ |- _ <  _ <= _ ] => split
+    | [ |- _ <= _ <= _ ] => split
+
+    | [ H : ?N < ?M |- ?N < ?M + ?O ] => apply (N.lt_lt_add_r _ _ _ H)
+    | [ H : 0 < ?M  |- ?N < ?N + ?M ] => apply (N.lt_add_pos_r _ _ H)
+
+    | [ H : context[Z.of_N (_ + _)] |- _ ] => rewrite N2Z.inj_add in H
+    | [ H : context[Z.of_N (_ - _)] |- _ ] => rewrite N2Z.inj_sub in H; trivial
+
+    | [ |- context[Z.of_N (_ + _)] ] => rewrite N2Z.inj_add
+    | [ |- context[Z.of_N (_ - _)] ] => rewrite N2Z.inj_sub
+
+    | [ H : _ = _ |- _ ] => subst
+
+    | [ H : context[_ < _]  |- _ ] => rewrite N2Z.inj_lt in H
+    (* | [ H : context[_ = _]  |- _ ] => apply N2Z.inj_iff in H *)
+    (* | [ H : context[_ <> _] |- _ ] => apply N2Z.inj_iff in H *)
+
+    (* We need to give _ <= _ alone a chance to be used by N2Z.inj_sub. *)
+    | [ H : context[_     <= _ + _] |- _ ] => rewrite N2Z.inj_le in H
+    | [ H : context[_ + _ <= _    ] |- _ ] => rewrite N2Z.inj_le in H
+    | [ H : context[_ + _ <= _ + _] |- _ ] => rewrite N2Z.inj_le in H
+    | [ H : context[_     <= _    ] |- _ ] => rewrite N2Z.inj_le in H
+
+    | [ |- context[_ < _]  ] => rewrite N2Z.inj_lt
+    | [ |- context[_ <= _] ] => rewrite N2Z.inj_le
+    | [ |- context[_ = _]  ] => apply N2Z.inj_iff
+    | [ |- context[_ <> _] ] => apply N2Z.inj_iff
+    end; undecide).
+
+Ltac nomega := solve [ nomega_reduce; abstract omega ].
+
+Lemma overlaps_within : forall addr1 len1 addr2 len2,
+  0 < len1 -> overlaps addr1 len1 addr2 len2
+                <-> IfDec addr1 < addr2
+                    Then within addr1 len1 addr2
+                    Else within addr2 len2 addr1.
+Proof.
+  unfold overlaps, within.
+  split; intros.
+    destruct H0.
+    decisions; nomega.
+  decisions;
+  destruct H0.
+    nomega.
+  split; trivial.
+  undecide.
+  apply N.lt_eq_cases in Heqe.
+  destruct Heqe; nomega.
+Qed.
+
+Corollary not_overlaps_within : forall addr1 len1 addr2 len2,
+  0 < len1 -> ~ overlaps addr1 len1 addr2 len2
+                <-> IfDec addr1 < addr2
+                    Then ~ within addr1 len1 addr2
+                    Else ~ within addr2 len2 addr1.
+Proof.
+  split; intros.
+    decisions;
+    unfold not; intros;
+    apply H0, overlaps_within; trivial;
+    decisions; firstorder.
+  unfold not; intros;
+  apply overlaps_within in H1; trivial;
+  decisions; firstorder.
+Qed.
+
+Theorem Nle_add_plus : forall n m o, 0 < o -> n <= m -> n <= m + o.
+Proof.
+  intros.
+  rewrite <- (N.add_0_r n).
+  apply N.add_le_mono; nomega.
+Qed.
+
+Theorem Nle_impossible : forall n m, 0 < m -> n + m <= n -> False.
+Proof.
+  intros.
+  rewrite <- (N.add_0_r n) in H0 at 2.
+  apply N.add_le_mono_l in H0.
+  nomega.
+Qed.
+
+Lemma within_reflect : forall x y a,
+  within x y a <-> ((x <=? a) && (a <? x + y) = true)%bool.
+Proof.
+  intros.
+  unfold within.
+  split; intros; try nomega.
+  apply Bool.andb_true_iff; split; nomega.
+Qed.
